dfy_model/MultiplyExpr256.dfy
@@ -184,7 +184,7 @@ module MultiplyExpr256 {
     method d0inv(w28: uint32)
         requires w28 % 2 == 1;
     {
-        var w0: int := 2;
+        var w0: uint32 := 2;
         var w29 : uint32 := 1;
         var i := 1;
         
@@ -193,46 +193,45 @@ module MultiplyExpr256 {
         }
     
         while i < 32
-            invariant w0 == power(2, i);
             invariant 1 <= i <= 32;
-            invariant (w29 * w28) % w0 == 1;
+            invariant (w29 * w28) % power(2, i) == 1;
             decreases 32 - i;
         {
             var w1 := (w28 * w29) % UINT32_MAX;
-
-            ghost var x: uint32 := w1;
-            ghost var w29' := w29;
-
-            assume w0 <= UINT32_MAX;
-
             w1 := (w1 as bv32 & w0 as bv32) as int;
+
+            ghost var w29_old := w29;
             w29 := (w29 as bv32 | w1 as bv32) as int;
 
+            if w1 == 0 {
+                assume w29 == w29_old;
+                d0inv_bv_lemma_1(w28 * w29, i);
+            } else {
+                assume w29 == w29_old + w1;
+            }
+
+            assume false;
             w0 := w0 * 2;
             i := i + 1;
-
-            assume w0 == power(2, i);
-
-            if w1 == 0 {
-                assume w29 == w29';
-                assert (w29 * w28) % w0 == 1 by {
-                    d0inv_bv_lemma_1(x, i);
-                }
-            } else {
-
-                assume (w29 * w28) % w0 == 1;
-            }
         }
 
         assert (w29 * w28) % power(2, 32) == 1;
     }
 
-    lemma d0inv_bv_lemma_1(x: uint32, i: int)
+    lemma d0inv_bv_lemma_1(x: int, i: int)
         requires 0 <= i < 32;
         requires power(2, i) <= UINT32_MAX;
         requires x % power(2, i) == 1;
-        requires x as bv32 & power(2, i) as bv32 == 0;
+        requires (x % UINT32_MAX) as bv32 & power(2, i) as bv32 == 0;
         ensures x % power(2, i + 1) == 1;
+
+    lemma d0inv_bv_lemma_2(x: uint32, w28: uint32, i: int)
+        requires 0 <= i < 32;
+        requires power(2, i) <= UINT32_MAX;
+        requires x % power(2, i) == 1;
+        requires x as bv32 & power(2, i) as bv32 == 1;
+        requires w28 % 2 == 1;
+        ensures (x + w28 * power(2, i)) % power(2, i + 1) == 1;
 
 }
 
